@prefix : <https://w3id.org/ontoforge/windprofle#> .
@prefix owl: <http://www.w3.org/2002/07/owl#> .
@prefix rdf: <http://www.w3.org/1999/02/22-rdf-syntax-ns#> .
@prefix xml: <http://www.w3.org/XML/1998/namespace> .
@prefix xsd: <http://www.w3.org/2001/XMLSchema#> .
@prefix rdfs: <http://www.w3.org/2000/01/rdf-schema#> .
@base <https://w3id.org/ontoforge/windprofle#> .

<https://w3id.org/ontoforge/windprofle#> rdf:type owl:Ontology ;
                                          <http://purl.org/dc/elements/1.1/publisher> <https://ost.ch/> ;
                                          <http://purl.org/dc/terms/creator> "IEA Wind Task 43"@en ;
                                          <http://purl.org/dc/terms/description> "A simple SKOS Taxonomy of a processes in wind energy according to the project life-cycle phases"@en ;
                                          <http://purl.org/dc/terms/issued> "2025-02-15"^^xsd:date ;
                                          <http://purl.org/dc/terms/license> <http://creativecommons.org/licenses/by/4.0/> ;
                                          <http://purl.org/dc/terms/modified> "2025-02-17"^^xsd:date ;
                                          <http://purl.org/dc/terms/publisher> <https://ost.ch> ;
                                          <http://purl.org/dc/terms/rights> "Copyright Â© 2025 OST Ostschweizer Fachhochschule" ;
                                          <http://purl.org/dc/terms/title> "Life Cycle Phase and Process Taxonomy"@en ;
                                          <http://purl.org/vocab/vann/preferredNamespacePrefix> "of-wpl" ;
                                          <http://purl.org/vocab/vann/preferredNamespaceUri> "https://w3id.org/ontoforge/windprofile#" ;
                                          rdfs:comment "This ontology aims to model a taxonomical organisation of a processes in wind energy according to the project life-cycle phases using a Simple Knoledge Organisation System (SKOS) data model."@en ;
                                          owl:versionInfo "0.1.2"@en ;
                                          <http://www.w3.org/2004/02/skos/core#hasTopConcept> <https://w3id.org/ontoforge/windprofile#LifeCyclePhase> ,
                                                                                              <https://w3id.org/ontoforge/windprofile#Process> ,
                                                                                              <https://w3id.org/ontoforge/windprofile#ProcessGroup> ;
                                          <http://www.w3.org/2004/02/skos/core#prefLabel> "WINDPROFILE"@en .

#################################################################
#    Annotation properties
#################################################################

###  http://purl.org/dc/elements/1.1/publisher
<http://purl.org/dc/elements/1.1/publisher> rdf:type owl:AnnotationProperty .


###  http://purl.org/dc/terms/bibliographicCitation
<http://purl.org/dc/terms/bibliographicCitation> rdf:type owl:AnnotationProperty .


###  http://purl.org/dc/terms/creator
<http://purl.org/dc/terms/creator> rdf:type owl:AnnotationProperty .


###  http://purl.org/dc/terms/description
<http://purl.org/dc/terms/description> rdf:type owl:AnnotationProperty .


###  http://purl.org/dc/terms/issued
<http://purl.org/dc/terms/issued> rdf:type owl:AnnotationProperty .


###  http://purl.org/dc/terms/license
<http://purl.org/dc/terms/license> rdf:type owl:AnnotationProperty .


###  http://purl.org/dc/terms/modified
<http://purl.org/dc/terms/modified> rdf:type owl:AnnotationProperty .


###  http://purl.org/dc/terms/publisher
<http://purl.org/dc/terms/publisher> rdf:type owl:AnnotationProperty .


###  http://purl.org/dc/terms/rights
<http://purl.org/dc/terms/rights> rdf:type owl:AnnotationProperty .


###  http://purl.org/dc/terms/title
<http://purl.org/dc/terms/title> rdf:type owl:AnnotationProperty .


###  http://purl.org/vocab/vann/preferredNamespacePrefix
<http://purl.org/vocab/vann/preferredNamespacePrefix> rdf:type owl:AnnotationProperty .


###  http://purl.org/vocab/vann/preferredNamespaceUri
<http://purl.org/vocab/vann/preferredNamespaceUri> rdf:type owl:AnnotationProperty .


###  http://www.w3.org/2004/02/skos/core#altLabel
<http://www.w3.org/2004/02/skos/core#altLabel> rdf:type owl:AnnotationProperty .


###  http://www.w3.org/2004/02/skos/core#broader
<http://www.w3.org/2004/02/skos/core#broader> rdf:type owl:AnnotationProperty .


###  http://www.w3.org/2004/02/skos/core#definition
<http://www.w3.org/2004/02/skos/core#definition> rdf:type owl:AnnotationProperty .


###  http://www.w3.org/2004/02/skos/core#hasTopConcept
<http://www.w3.org/2004/02/skos/core#hasTopConcept> rdf:type owl:AnnotationProperty .


###  http://www.w3.org/2004/02/skos/core#inScheme
<http://www.w3.org/2004/02/skos/core#inScheme> rdf:type owl:AnnotationProperty .


###  http://www.w3.org/2004/02/skos/core#narrower
<http://www.w3.org/2004/02/skos/core#narrower> rdf:type owl:AnnotationProperty .


###  http://www.w3.org/2004/02/skos/core#prefLabel
<http://www.w3.org/2004/02/skos/core#prefLabel> rdf:type owl:AnnotationProperty .


###  http://www.w3.org/2004/02/skos/core#topConceptOf
<http://www.w3.org/2004/02/skos/core#topConceptOf> rdf:type owl:AnnotationProperty .


#################################################################
#    Datatypes
#################################################################

###  http://www.w3.org/2001/XMLSchema#date
xsd:date rdf:type rdfs:Datatype .


#################################################################
#    Classes
#################################################################

###  http://www.w3.org/2004/02/skos/core#Concept
<http://www.w3.org/2004/02/skos/core#Concept> rdf:type owl:Class .


###  http://www.w3.org/2004/02/skos/core#ConceptScheme
<http://www.w3.org/2004/02/skos/core#ConceptScheme> rdf:type owl:Class .


#################################################################
#    Individuals
#################################################################

###  https://w3id.org/ontoforge/windprofile#AllProductPhases
<https://w3id.org/ontoforge/windprofile#AllProductPhases> rdf:type owl:NamedIndividual ,
                                                                   <http://www.w3.org/2004/02/skos/core#Concept> ;
                                                          <http://www.w3.org/2004/02/skos/core#broader> <https://w3id.org/ontoforge/windprofile#ProductLife-cyclePhase> ;
                                                          <http://www.w3.org/2004/02/skos/core#inScheme> <https://w3id.org/ontoforge/windprofile#> ;
                                                          <http://www.w3.org/2004/02/skos/core#prefLabel> "All Product Phases"@en .


###  https://w3id.org/ontoforge/windprofile#AllProjectPhases
<https://w3id.org/ontoforge/windprofile#AllProjectPhases> rdf:type owl:NamedIndividual ,
                                                                   <http://www.w3.org/2004/02/skos/core#Concept> ;
                                                          <http://www.w3.org/2004/02/skos/core#broader> <https://w3id.org/ontoforge/windprofile#ReferenceProjectLife-cyclePhase> ;
                                                          <http://www.w3.org/2004/02/skos/core#inScheme> <https://w3id.org/ontoforge/windprofile#> ;
                                                          <http://www.w3.org/2004/02/skos/core#prefLabel> "All Project Phases"@en .


###  https://w3id.org/ontoforge/windprofile#Build
<https://w3id.org/ontoforge/windprofile#Build> rdf:type owl:NamedIndividual ,
                                                        <http://www.w3.org/2004/02/skos/core#Concept> ;
                                               <http://purl.org/dc/terms/bibliographicCitation> "urn:ISBN:9781628256659"@en ;
                                               <http://purl.org/dc/terms/creator> <https://www.pmi.org/> ;
                                               <http://www.w3.org/2004/02/skos/core#broader> <https://w3id.org/ontoforge/windprofile#ReferenceProjectLife-cyclePhase> ;
                                               <http://www.w3.org/2004/02/skos/core#definition> "Construction of the deliverable with integrated quality assurance activities is conducted."@en ;
                                               <http://www.w3.org/2004/02/skos/core#inScheme> <https://w3id.org/ontoforge/windprofile#> ;
                                               <http://www.w3.org/2004/02/skos/core#prefLabel> "Build"@en .


###  https://w3id.org/ontoforge/windprofile#Close
<https://w3id.org/ontoforge/windprofile#Close> rdf:type owl:NamedIndividual ,
                                                        <http://www.w3.org/2004/02/skos/core#Concept> ;
                                               <http://purl.org/dc/terms/bibliographicCitation> "urn:ISBN:9781628256659"@en ;
                                               <http://purl.org/dc/terms/creator> <https://www.pmi.org/> ;
                                               <http://www.w3.org/2004/02/skos/core#broader> <https://w3id.org/ontoforge/windprofile#ReferenceProjectLife-cyclePhase> ;
                                               <http://www.w3.org/2004/02/skos/core#definition> "The project is closed, project knowledge and artifacts are archived, project team members are released, and contracts are closed."@en ;
                                               <http://www.w3.org/2004/02/skos/core#inScheme> <https://w3id.org/ontoforge/windprofile#> ;
                                               <http://www.w3.org/2004/02/skos/core#prefLabel> "Close"@en .


###  https://w3id.org/ontoforge/windprofile#Closure
<https://w3id.org/ontoforge/windprofile#Closure> rdf:type owl:NamedIndividual ,
                                                          <http://www.w3.org/2004/02/skos/core#Concept> ;
                                                 <http://purl.org/dc/terms/bibliographicCitation> "urn:ISBN:9781628256659"@en ;
                                                 <http://purl.org/dc/terms/creator> <https://www.pmi.org/> ;
                                                 <http://www.w3.org/2004/02/skos/core#broader> <https://w3id.org/ontoforge/windprofile#ProcessGroup> ;
                                                 <http://www.w3.org/2004/02/skos/core#definition> "Those processes performed to formally complete or close a project, phase, or contract."@en ;
                                                 <http://www.w3.org/2004/02/skos/core#inScheme> <https://w3id.org/ontoforge/windprofile#> ;
                                                 <http://www.w3.org/2004/02/skos/core#prefLabel> "Closure"@en .


###  https://w3id.org/ontoforge/windprofile#Conception
<https://w3id.org/ontoforge/windprofile#Conception> rdf:type owl:NamedIndividual ,
                                                             <http://www.w3.org/2004/02/skos/core#Concept> ;
                                                    <http://www.w3.org/2004/02/skos/core#broader> <https://w3id.org/ontoforge/windprofile#ProductLife-cyclePhase> ;
                                                    <http://www.w3.org/2004/02/skos/core#inScheme> <https://w3id.org/ontoforge/windprofile#> ;
                                                    <http://www.w3.org/2004/02/skos/core#prefLabel> "Conception"@en .


###  https://w3id.org/ontoforge/windprofile#Deploy
<https://w3id.org/ontoforge/windprofile#Deploy> rdf:type owl:NamedIndividual ,
                                                         <http://www.w3.org/2004/02/skos/core#Concept> ;
                                                <http://purl.org/dc/terms/bibliographicCitation> "urn:ISBN:9781628256659"@en ;
                                                <http://purl.org/dc/terms/creator> <https://www.pmi.org/> ;
                                                <http://www.w3.org/2004/02/skos/core#broader> <https://w3id.org/ontoforge/windprofile#ReferenceProjectLife-cyclePhase> ;
                                                <http://www.w3.org/2004/02/skos/core#definition> "Project deliverables are put into use and transitional activities required for sustainment, benefits realization, and organizational change management are completed."@en ;
                                                <http://www.w3.org/2004/02/skos/core#inScheme> <https://w3id.org/ontoforge/windprofile#> ;
                                                <http://www.w3.org/2004/02/skos/core#prefLabel> "Deploy"@en .


###  https://w3id.org/ontoforge/windprofile#Design
<https://w3id.org/ontoforge/windprofile#Design> rdf:type owl:NamedIndividual ,
                                                         <http://www.w3.org/2004/02/skos/core#Concept> ;
                                                <http://purl.org/dc/terms/bibliographicCitation> "urn:ISBN:9781628256659"@en ;
                                                <http://purl.org/dc/terms/creator> <https://www.pmi.org/> ;
                                                <http://www.w3.org/2004/02/skos/core#broader> <https://w3id.org/ontoforge/windprofile#ProductLife-cyclePhase> ,
                                                                                              <https://w3id.org/ontoforge/windprofile#ReferenceProjectLife-cyclePhase> ;
                                                <http://www.w3.org/2004/02/skos/core#definition> "Planning and analysis lead to the design of the project deliverable that will be developed."@en ;
                                                <http://www.w3.org/2004/02/skos/core#inScheme> <https://w3id.org/ontoforge/windprofile#> ;
                                                <http://www.w3.org/2004/02/skos/core#prefLabel> "Design"@en .


###  https://w3id.org/ontoforge/windprofile#Execution
<https://w3id.org/ontoforge/windprofile#Execution> rdf:type owl:NamedIndividual ,
                                                            <http://www.w3.org/2004/02/skos/core#Concept> ;
                                                   <http://purl.org/dc/terms/bibliographicCitation> "urn:ISBN:9781628256659"@en ;
                                                   <http://purl.org/dc/terms/creator> <https://www.pmi.org/> ;
                                                   <http://www.w3.org/2004/02/skos/core#altLabel> "Implementation"@en ;
                                                   <http://www.w3.org/2004/02/skos/core#broader> <https://w3id.org/ontoforge/windprofile#ProcessGroup> ;
                                                   <http://www.w3.org/2004/02/skos/core#definition> "Those processes performed to complete the work defined in the project management plan to satisfy the project requirements."@en ;
                                                   <http://www.w3.org/2004/02/skos/core#inScheme> <https://w3id.org/ontoforge/windprofile#> ;
                                                   <http://www.w3.org/2004/02/skos/core#prefLabel> "Execution"@en .


###  https://w3id.org/ontoforge/windprofile#Feasibility
<https://w3id.org/ontoforge/windprofile#Feasibility> rdf:type owl:NamedIndividual ,
                                                              <http://www.w3.org/2004/02/skos/core#Concept> ;
                                                     <http://purl.org/dc/terms/bibliographicCitation> "urn:ISBN:9781628256659"@en ;
                                                     <http://purl.org/dc/terms/creator> <https://www.pmi.org/> ;
                                                     <http://www.w3.org/2004/02/skos/core#broader> <https://w3id.org/ontoforge/windprofile#ReferenceProjectLife-cyclePhase> ;
                                                     <http://www.w3.org/2004/02/skos/core#definition> "This phase determines if the business case is valid and if the organization has the capability to deliver the intended outcome."@en ;
                                                     <http://www.w3.org/2004/02/skos/core#inScheme> <https://w3id.org/ontoforge/windprofile#> ;
                                                     <http://www.w3.org/2004/02/skos/core#prefLabel> "Feasibility"@en .


###  https://w3id.org/ontoforge/windprofile#Initiation
<https://w3id.org/ontoforge/windprofile#Initiation> rdf:type owl:NamedIndividual ,
                                                             <http://www.w3.org/2004/02/skos/core#Concept> ;
                                                    <http://purl.org/dc/terms/bibliographicCitation> "urn:ISBN:9781628256659"@en ;
                                                    <http://purl.org/dc/terms/creator> <https://www.pmi.org/> ;
                                                    <http://www.w3.org/2004/02/skos/core#broader> <https://w3id.org/ontoforge/windprofile#ProcessGroup> ;
                                                    <http://www.w3.org/2004/02/skos/core#definition> "Those processes performed to define a new project or a new phase of an existing project by obtaining authorization to start the project or phase."@en ;
                                                    <http://www.w3.org/2004/02/skos/core#inScheme> <https://w3id.org/ontoforge/windprofile#> ;
                                                    <http://www.w3.org/2004/02/skos/core#prefLabel> "Initiation"@en .


###  https://w3id.org/ontoforge/windprofile#LifeCyclePhase
<https://w3id.org/ontoforge/windprofile#LifeCyclePhase> rdf:type owl:NamedIndividual ,
                                                                 <http://www.w3.org/2004/02/skos/core#Concept> ;
                                                        <http://www.w3.org/2004/02/skos/core#inScheme> <https://w3id.org/ontoforge/windprofile#> ;
                                                        <http://www.w3.org/2004/02/skos/core#narrower> <https://w3id.org/ontoforge/windprofile#ProductLife-cyclePhase> ,
                                                                                                       <https://w3id.org/ontoforge/windprofile#ReferenceProjectLife-cyclePhase> ,
                                                                                                       <https://w3id.org/ontoforge/windprofile#WindEnergyProjectLife-cyclePhase> ;
                                                        <http://www.w3.org/2004/02/skos/core#prefLabel> "Life Cycle Phase"@en ;
                                                        <http://www.w3.org/2004/02/skos/core#topConceptOf> <https://w3id.org/ontoforge/windprofile#> .


###  https://w3id.org/ontoforge/windprofile#Performance-Control
<https://w3id.org/ontoforge/windprofile#Performance-Control> rdf:type owl:NamedIndividual ,
                                                                      <http://www.w3.org/2004/02/skos/core#Concept> ;
                                                             <http://purl.org/dc/terms/bibliographicCitation> "urn:ISBN:9781628256659"@en ;
                                                             <http://purl.org/dc/terms/creator> <https://www.pmi.org/> ;
                                                             <http://www.w3.org/2004/02/skos/core#broader> <https://w3id.org/ontoforge/windprofile#ProcessGroup> ;
                                                             <http://www.w3.org/2004/02/skos/core#definition> "Those processes required to track, review, and regulate the progress and performance of the project; identify any areas in which changes to the plan are required; and initiate the corresponding changes."@en ;
                                                             <http://www.w3.org/2004/02/skos/core#inScheme> <https://w3id.org/ontoforge/windprofile#> ;
                                                             <http://www.w3.org/2004/02/skos/core#prefLabel> "Performance & Control"@en .


###  https://w3id.org/ontoforge/windprofile#Planning
<https://w3id.org/ontoforge/windprofile#Planning> rdf:type owl:NamedIndividual ,
                                                           <http://www.w3.org/2004/02/skos/core#Concept> ;
                                                  <http://purl.org/dc/terms/bibliographicCitation> "urn:ISBN:9781628256659"@en ;
                                                  <http://purl.org/dc/terms/creator> <https://www.pmi.org/> ;
                                                  <http://www.w3.org/2004/02/skos/core#broader> <https://w3id.org/ontoforge/windprofile#ProcessGroup> ;
                                                  <http://www.w3.org/2004/02/skos/core#definition> "Those processes required to establish the scope of the project, refine the objectives, and define the course of action required to attain the objectives that the project was undertaken to achieve."@en ;
                                                  <http://www.w3.org/2004/02/skos/core#inScheme> <https://w3id.org/ontoforge/windprofile#> ;
                                                  <http://www.w3.org/2004/02/skos/core#prefLabel> "Planning"@en .


###  https://w3id.org/ontoforge/windprofile#Process
<https://w3id.org/ontoforge/windprofile#Process> rdf:type owl:NamedIndividual ,
                                                          <http://www.w3.org/2004/02/skos/core#Concept> ;
                                                 <http://www.w3.org/2004/02/skos/core#inScheme> <https://w3id.org/ontoforge/windprofile#> ;
                                                 <http://www.w3.org/2004/02/skos/core#narrower> <https://w3id.org/ontoforge/windprofile#ProductProcess> ,
                                                                                                <https://w3id.org/ontoforge/windprofile#ProjectManagementProcess> ,
                                                                                                <https://w3id.org/ontoforge/windprofile#SupportingProcess> ;
                                                 <http://www.w3.org/2004/02/skos/core#prefLabel> "Process"@en ;
                                                 <http://www.w3.org/2004/02/skos/core#topConceptOf> <https://w3id.org/ontoforge/windprofile#> .


###  https://w3id.org/ontoforge/windprofile#ProcessGroup
<https://w3id.org/ontoforge/windprofile#ProcessGroup> rdf:type owl:NamedIndividual ,
                                                               <http://www.w3.org/2004/02/skos/core#Concept> ;
                                                      <http://purl.org/dc/terms/bibliographicCitation> "urn:ISBN:9781628256659"@en ;
                                                      <http://purl.org/dc/terms/creator> <https://www.pmi.org/> ;
                                                      <http://www.w3.org/2004/02/skos/core#definition> "Projects that follow a process-based approach may adopt project process groups. Project management processes can be organized into logical groupings of project management inputs, tools and techniques, and outputs that are tailored to meet the needs of the organization, stakeholders, and the project. Groups of processes are not project phases. The Process Groups interact within each phase of a project life cycle. In a process-based approach, the output of one process generally becomes an input to another process or is a deliverable of the project or project phase."@en ;
                                                      <http://www.w3.org/2004/02/skos/core#inScheme> <https://w3id.org/ontoforge/windprofile#> ;
                                                      <http://www.w3.org/2004/02/skos/core#narrower> <https://w3id.org/ontoforge/windprofile#Closure> ,
                                                                                                     <https://w3id.org/ontoforge/windprofile#Execution> ,
                                                                                                     <https://w3id.org/ontoforge/windprofile#Initiation> ,
                                                                                                     <https://w3id.org/ontoforge/windprofile#Performance-Control> ,
                                                                                                     <https://w3id.org/ontoforge/windprofile#Planning> ;
                                                      <http://www.w3.org/2004/02/skos/core#prefLabel> "Process Group"@en ;
                                                      <http://www.w3.org/2004/02/skos/core#topConceptOf> <https://w3id.org/ontoforge/windprofile#> .


###  https://w3id.org/ontoforge/windprofile#ProductLife-cyclePhase
<https://w3id.org/ontoforge/windprofile#ProductLife-cyclePhase> rdf:type owl:NamedIndividual ,
                                                                         <http://www.w3.org/2004/02/skos/core#Concept> ;
                                                                <http://www.w3.org/2004/02/skos/core#broader> <https://w3id.org/ontoforge/windprofile#LifeCyclePhase> ;
                                                                <http://www.w3.org/2004/02/skos/core#inScheme> <https://w3id.org/ontoforge/windprofile#> ;
                                                                <http://www.w3.org/2004/02/skos/core#narrower> <https://w3id.org/ontoforge/windprofile#AllProductPhases> ,
                                                                                                               <https://w3id.org/ontoforge/windprofile#Conception> ,
                                                                                                               <https://w3id.org/ontoforge/windprofile#Design> ,
                                                                                                               <https://w3id.org/ontoforge/windprofile#Realisation> ,
                                                                                                               <https://w3id.org/ontoforge/windprofile#Service> ;
                                                                <http://www.w3.org/2004/02/skos/core#prefLabel> "Product Life-cycle Phase"@en .


###  https://w3id.org/ontoforge/windprofile#ProductProcess
<https://w3id.org/ontoforge/windprofile#ProductProcess> rdf:type owl:NamedIndividual ,
                                                                 <http://www.w3.org/2004/02/skos/core#Concept> ;
                                                        <http://www.w3.org/2004/02/skos/core#altLabel> "Delivery Process"@en ;
                                                        <http://www.w3.org/2004/02/skos/core#broader> <https://w3id.org/ontoforge/windprofile#Process> ;
                                                        <http://www.w3.org/2004/02/skos/core#definition> "Product process is not unique to project management, which results in the specification and provision of a particular product, service or result, and which varies depending on the particular project deliverable."@en ;
                                                        <http://www.w3.org/2004/02/skos/core#inScheme> <https://w3id.org/ontoforge/windprofile#> ;
                                                        <http://www.w3.org/2004/02/skos/core#narrower> <https://w3id.org/ontoforge/windprofile#WindPowerPlantProcess> ,
                                                                                                       <https://w3id.org/ontoforge/windprofile#WindTurbineProductProcess> ;
                                                        <http://www.w3.org/2004/02/skos/core#prefLabel> "Product Process"@en .


###  https://w3id.org/ontoforge/windprofile#ProjectManagementProcess
<https://w3id.org/ontoforge/windprofile#ProjectManagementProcess> rdf:type owl:NamedIndividual ,
                                                                           <http://www.w3.org/2004/02/skos/core#Concept> ;
                                                                  <http://www.w3.org/2004/02/skos/core#broader> <https://w3id.org/ontoforge/windprofile#Process> ;
                                                                  <http://www.w3.org/2004/02/skos/core#definition> "Project management process is specific to project management. It determines how the activities selected for the project are managed."@en ;
                                                                  <http://www.w3.org/2004/02/skos/core#inScheme> <https://w3id.org/ontoforge/windprofile#> ;
                                                                  <http://www.w3.org/2004/02/skos/core#prefLabel> "Project Management Process"@en .


###  https://w3id.org/ontoforge/windprofile#Realisation
<https://w3id.org/ontoforge/windprofile#Realisation> rdf:type owl:NamedIndividual ,
                                                              <http://www.w3.org/2004/02/skos/core#Concept> ;
                                                     <http://www.w3.org/2004/02/skos/core#broader> <https://w3id.org/ontoforge/windprofile#ProductLife-cyclePhase> ;
                                                     <http://www.w3.org/2004/02/skos/core#inScheme> <https://w3id.org/ontoforge/windprofile#> ;
                                                     <http://www.w3.org/2004/02/skos/core#prefLabel> "Realisation"@en .


###  https://w3id.org/ontoforge/windprofile#ReferenceProjectLife-cyclePhase
<https://w3id.org/ontoforge/windprofile#ReferenceProjectLife-cyclePhase> rdf:type owl:NamedIndividual ,
                                                                                  <http://www.w3.org/2004/02/skos/core#Concept> ;
                                                                         <http://purl.org/dc/terms/bibliographicCitation> "urn:ISBN:9781628256659"@en ;
                                                                         <http://purl.org/dc/terms/creator> <https://www.pmi.org/> ;
                                                                         <http://www.w3.org/2004/02/skos/core#broader> <https://w3id.org/ontoforge/windprofile#LifeCyclePhase> ;
                                                                         <http://www.w3.org/2004/02/skos/core#definition> "Project phase is a collection of logically related project activities (processes) that culminates in the completion of one or more deliverables. Project Life Cycle is the series of phases that a project passes through from its start to its completion."@en ;
                                                                         <http://www.w3.org/2004/02/skos/core#inScheme> <https://w3id.org/ontoforge/windprofile#> ;
                                                                         <http://www.w3.org/2004/02/skos/core#narrower> <https://w3id.org/ontoforge/windprofile#AllProjectPhases> ,
                                                                                                                        <https://w3id.org/ontoforge/windprofile#Build> ,
                                                                                                                        <https://w3id.org/ontoforge/windprofile#Close> ,
                                                                                                                        <https://w3id.org/ontoforge/windprofile#Deploy> ,
                                                                                                                        <https://w3id.org/ontoforge/windprofile#Design> ,
                                                                                                                        <https://w3id.org/ontoforge/windprofile#Feasibility> ,
                                                                                                                        <https://w3id.org/ontoforge/windprofile#Test> ;
                                                                         <http://www.w3.org/2004/02/skos/core#prefLabel> "Reference Project Life-cycle Phase"@en .


###  https://w3id.org/ontoforge/windprofile#Service
<https://w3id.org/ontoforge/windprofile#Service> rdf:type owl:NamedIndividual ,
                                                          <http://www.w3.org/2004/02/skos/core#Concept> ;
                                                 <http://www.w3.org/2004/02/skos/core#broader> <https://w3id.org/ontoforge/windprofile#ProductLife-cyclePhase> ;
                                                 <http://www.w3.org/2004/02/skos/core#inScheme> <https://w3id.org/ontoforge/windprofile#> ;
                                                 <http://www.w3.org/2004/02/skos/core#prefLabel> "Service"@en .


###  https://w3id.org/ontoforge/windprofile#SupportingProcess
<https://w3id.org/ontoforge/windprofile#SupportingProcess> rdf:type owl:NamedIndividual ,
                                                                    <http://www.w3.org/2004/02/skos/core#Concept> ;
                                                           <http://www.w3.org/2004/02/skos/core#altLabel> "Cross-cutting Process"@en ,
                                                                                                          "Supporting Activities"@en ;
                                                           <http://www.w3.org/2004/02/skos/core#broader> <https://w3id.org/ontoforge/windprofile#Process> ;
                                                           <http://www.w3.org/2004/02/skos/core#definition> "Supporting process is a process not unique to project management and which provides relevant and valuable support to product and project management processes in such disciplines as logistics, finance, accounting and safety."@en ;
                                                           <http://www.w3.org/2004/02/skos/core#inScheme> <https://w3id.org/ontoforge/windprofile#> ;
                                                           <http://www.w3.org/2004/02/skos/core#prefLabel> "Supporting Process"@en .


###  https://w3id.org/ontoforge/windprofile#Test
<https://w3id.org/ontoforge/windprofile#Test> rdf:type owl:NamedIndividual ,
                                                       <http://www.w3.org/2004/02/skos/core#Concept> ;
                                              <http://purl.org/dc/terms/bibliographicCitation> "urn:ISBN:9781628256659"@en ;
                                              <http://purl.org/dc/terms/creator> <https://www.pmi.org/> ;
                                              <http://www.w3.org/2004/02/skos/core#broader> <https://w3id.org/ontoforge/windprofile#ReferenceProjectLife-cyclePhase> ;
                                              <http://www.w3.org/2004/02/skos/core#definition> "Final quality review and inspection of deliverables are carried out before transition, go-live, or acceptance by the customer."@en ;
                                              <http://www.w3.org/2004/02/skos/core#inScheme> <https://w3id.org/ontoforge/windprofile#> ;
                                              <http://www.w3.org/2004/02/skos/core#prefLabel> "Test"@en .


###  https://w3id.org/ontoforge/windprofile#WindEnergyProjectLife-cyclePhase
<https://w3id.org/ontoforge/windprofile#WindEnergyProjectLife-cyclePhase> rdf:type owl:NamedIndividual ,
                                                                                   <http://www.w3.org/2004/02/skos/core#Concept> ;
                                                                          <http://www.w3.org/2004/02/skos/core#broader> <https://w3id.org/ontoforge/windprofile#LifeCyclePhase> ;
                                                                          <http://www.w3.org/2004/02/skos/core#inScheme> <https://w3id.org/ontoforge/windprofile#> ;
                                                                          <http://www.w3.org/2004/02/skos/core#narrower> <https://w3id.org/ontoforge/windprofile#1Identification> ,
                                                                                                                         <https://w3id.org/ontoforge/windprofile#2Feasibility> ,
                                                                                                                         <https://w3id.org/ontoforge/windprofile#3Development> ,
                                                                                                                         <https://w3id.org/ontoforge/windprofile#4Pre-Construction> ,
                                                                                                                         <https://w3id.org/ontoforge/windprofile#5Construction> ,
                                                                                                                         <https://w3id.org/ontoforge/windprofile#6Commissioning> ,
                                                                                                                         <https://w3id.org/ontoforge/windprofile#7Operation-Maintenance> ,
                                                                                                                         <https://w3id.org/ontoforge/windprofile#8Decommissioning> ;
                                                                          <http://www.w3.org/2004/02/skos/core#prefLabel> "Wind Energy Project Life-cycle Phase"@en .


###  https://w3id.org/ontoforge/windprofile#WindPowerPlantProcess
<https://w3id.org/ontoforge/windprofile#WindPowerPlantProcess> rdf:type owl:NamedIndividual ,
                                                                        <http://www.w3.org/2004/02/skos/core#Concept> ;
                                                               <http://www.w3.org/2004/02/skos/core#broader> <https://w3id.org/ontoforge/windprofile#ProductProcess> ;
                                                               <http://www.w3.org/2004/02/skos/core#inScheme> <https://w3id.org/ontoforge/windprofile#> ;
                                                               <http://www.w3.org/2004/02/skos/core#prefLabel> "Wind Power Plant Process"@en .


###  https://w3id.org/ontoforge/windprofile#WindTurbineProductProcess
<https://w3id.org/ontoforge/windprofile#WindTurbineProductProcess> rdf:type owl:NamedIndividual ,
                                                                            <http://www.w3.org/2004/02/skos/core#Concept> ;
                                                                   <http://www.w3.org/2004/02/skos/core#broader> <https://w3id.org/ontoforge/windprofile#ProductProcess> ;
                                                                   <http://www.w3.org/2004/02/skos/core#inScheme> <https://w3id.org/ontoforge/windprofile#> ;
                                                                   <http://www.w3.org/2004/02/skos/core#prefLabel> "Wind Turbine Product Process"@en .


###  https://w3id.org/ontoforge/windprofile#1Identification
<https://w3id.org/ontoforge/windprofile#1Identification> rdf:type owl:NamedIndividual ,
                                                                  <http://www.w3.org/2004/02/skos/core#Concept> ;
                                                         <http://www.w3.org/2004/02/skos/core#altLabel> "Pilot Study"@en ,
                                                                                                        "Screening"@en ,
                                                                                                        "Site Selection"@en ;
                                                         <http://www.w3.org/2004/02/skos/core#broader> <https://w3id.org/ontoforge/windprofile#WindEnergyProjectLife-cyclePhase> ;
                                                         <http://www.w3.org/2004/02/skos/core#definition> "Initial stage where potential wind energy sites are identified based on criteria like wind resource, land availability, and environmental factors."@en ;
                                                         <http://www.w3.org/2004/02/skos/core#inScheme> <https://w3id.org/ontoforge/windprofile#> ;
                                                         <http://www.w3.org/2004/02/skos/core#prefLabel> "1 Identification"@en .


###  https://w3id.org/ontoforge/windprofile#2Feasibility
<https://w3id.org/ontoforge/windprofile#2Feasibility> rdf:type owl:NamedIndividual ,
                                                               <http://www.w3.org/2004/02/skos/core#Concept> ;
                                                      <http://www.w3.org/2004/02/skos/core#broader> <https://w3id.org/ontoforge/windprofile#WindEnergyProjectLife-cyclePhase> ;
                                                      <http://www.w3.org/2004/02/skos/core#definition> "Detailed analysis of the identified site, including technical, environmental, and financial assessments to determine project viability."@en ;
                                                      <http://www.w3.org/2004/02/skos/core#inScheme> <https://w3id.org/ontoforge/windprofile#> ;
                                                      <http://www.w3.org/2004/02/skos/core#prefLabel> "2 Feasibility"@en .


###  https://w3id.org/ontoforge/windprofile#3Development
<https://w3id.org/ontoforge/windprofile#3Development> rdf:type owl:NamedIndividual ,
                                                               <http://www.w3.org/2004/02/skos/core#Concept> ;
                                                      <http://www.w3.org/2004/02/skos/core#altLabel> "Design"@en ,
                                                                                                     "Planning & Permitting"@en ;
                                                      <http://www.w3.org/2004/02/skos/core#broader> <https://w3id.org/ontoforge/windprofile#WindEnergyProjectLife-cyclePhase> ;
                                                      <http://www.w3.org/2004/02/skos/core#definition> "Preparation of detailed plans and engineering designs, wind turbine technology and vendor selection, securing permits, land leases, financing, and stakeholder agreements required to move forward with the project."@en ;
                                                      <http://www.w3.org/2004/02/skos/core#inScheme> <https://w3id.org/ontoforge/windprofile#> ;
                                                      <http://www.w3.org/2004/02/skos/core#prefLabel> "3 Development"@en .


###  https://w3id.org/ontoforge/windprofile#4Pre-Construction
<https://w3id.org/ontoforge/windprofile#4Pre-Construction> rdf:type owl:NamedIndividual ,
                                                                    <http://www.w3.org/2004/02/skos/core#Concept> ;
                                                           <http://www.w3.org/2004/02/skos/core#altLabel> "Procurement"@en ,
                                                                                                          "Purchase"@en ;
                                                           <http://www.w3.org/2004/02/skos/core#broader> <https://w3id.org/ontoforge/windprofile#WindEnergyProjectLife-cyclePhase> ;
                                                           <http://www.w3.org/2004/02/skos/core#definition> "Finalizing detailed engineering designs, procurement of materials, and preparation of the site for construction, including contractor selection."@en ;
                                                           <http://www.w3.org/2004/02/skos/core#inScheme> <https://w3id.org/ontoforge/windprofile#> ;
                                                           <http://www.w3.org/2004/02/skos/core#prefLabel> "4 Pre-Construction"@en .


###  https://w3id.org/ontoforge/windprofile#5Construction
<https://w3id.org/ontoforge/windprofile#5Construction> rdf:type owl:NamedIndividual ,
                                                                <http://www.w3.org/2004/02/skos/core#Concept> ;
                                                       <http://www.w3.org/2004/02/skos/core#broader> <https://w3id.org/ontoforge/windprofile#WindEnergyProjectLife-cyclePhase> ;
                                                       <http://www.w3.org/2004/02/skos/core#definition> "Physical construction of the wind farm, including infrastructure setup (turbines, roads, electrical connections) and project management oversight."@en ;
                                                       <http://www.w3.org/2004/02/skos/core#inScheme> <https://w3id.org/ontoforge/windprofile#> ;
                                                       <http://www.w3.org/2004/02/skos/core#prefLabel> "5 Construction"@en .


###  https://w3id.org/ontoforge/windprofile#6Commissioning
<https://w3id.org/ontoforge/windprofile#6Commissioning> rdf:type owl:NamedIndividual ,
                                                                 <http://www.w3.org/2004/02/skos/core#Concept> ;
                                                        <http://www.w3.org/2004/02/skos/core#broader> <https://w3id.org/ontoforge/windprofile#WindEnergyProjectLife-cyclePhase> ;
                                                        <http://www.w3.org/2004/02/skos/core#definition> "Testing and certifying that the wind farm operates according to design specifications before becoming fully operational."@en ;
                                                        <http://www.w3.org/2004/02/skos/core#inScheme> <https://w3id.org/ontoforge/windprofile#> ;
                                                        <http://www.w3.org/2004/02/skos/core#prefLabel> "6 Commissioning"@en .


###  https://w3id.org/ontoforge/windprofile#7Operation-Maintenance
<https://w3id.org/ontoforge/windprofile#7Operation-Maintenance> rdf:type owl:NamedIndividual ,
                                                                         <http://www.w3.org/2004/02/skos/core#Concept> ;
                                                                <http://www.w3.org/2004/02/skos/core#altLabel> "Middle of life"@en ;
                                                                <http://www.w3.org/2004/02/skos/core#broader> <https://w3id.org/ontoforge/windprofile#WindEnergyProjectLife-cyclePhase> ;
                                                                <http://www.w3.org/2004/02/skos/core#definition> "Ongoing operation of the wind farm, including regular monitoring, maintenance, and optimization to ensure maximum energy production and efficiency."@en ;
                                                                <http://www.w3.org/2004/02/skos/core#inScheme> <https://w3id.org/ontoforge/windprofile#> ;
                                                                <http://www.w3.org/2004/02/skos/core#prefLabel> "7 Operation & Maintenance"@en .


###  https://w3id.org/ontoforge/windprofile#8Decommissioning
<https://w3id.org/ontoforge/windprofile#8Decommissioning> rdf:type owl:NamedIndividual ,
                                                                   <http://www.w3.org/2004/02/skos/core#Concept> ;
                                                          <http://www.w3.org/2004/02/skos/core#altLabel> "End of life"@en ;
                                                          <http://www.w3.org/2004/02/skos/core#broader> <https://w3id.org/ontoforge/windprofile#WindEnergyProjectLife-cyclePhase> ;
                                                          <http://www.w3.org/2004/02/skos/core#definition> "End-of-life activities for the wind farm, involving dismantling turbines and infrastructure, restoring the site, and recycling or disposing of materials."@en ;
                                                          <http://www.w3.org/2004/02/skos/core#inScheme> <https://w3id.org/ontoforge/windprofile#> ;
                                                          <http://www.w3.org/2004/02/skos/core#prefLabel> "8 Decommissioning"@en .


###  https://w3id.org/ontoforge/windprofle#
<https://w3id.org/ontoforge/windprofle#> rdf:type owl:NamedIndividual ,
                                                  <http://www.w3.org/2004/02/skos/core#ConceptScheme> .


###  Generated by the OWL API (version 5.1.18) https://github.com/owlcs/owlapi/
