@prefix : <https://w3id.org/ontoforge/bdo#> .
@prefix owl: <http://www.w3.org/2002/07/owl#> .
@prefix rdf: <http://www.w3.org/1999/02/22-rdf-syntax-ns#> .
@prefix xml: <http://www.w3.org/XML/1998/namespace> .
@prefix xsd: <http://www.w3.org/2001/XMLSchema#> .
@prefix rdfs: <http://www.w3.org/2000/01/rdf-schema#> .
@base <https://w3id.org/ontoforge/bdo#> .

<https://w3id.org/ontoforge/bdo#> rdf:type owl:Ontology ;
                                   <http://purl.org/dc/terms/creator> <https://w3id.org/people/jpcik/me> ;
                                   <http://purl.org/dc/terms/description> "This ontology aims to model Blade damage based on a white paper by EPRI. The ontology is developed in the context of the xxxx project"@en ;
                                   <http://purl.org/dc/terms/issued> "2025-02-15"^^xsd:date ;
                                   <http://purl.org/dc/terms/license> <https://creativecommons.org/licenses/by/4.0/> ;
                                   <http://purl.org/dc/terms/modified> "2025-02-17"^^xsd:date ;
                                   <http://purl.org/dc/terms/publisher> <https://ost.ch> ,
                                                                        <https://ost.ch/> ;
                                   <http://purl.org/dc/terms/rights> "Copyright Â© 2025 OST Ostschweizer Fachhochschule" ;
                                   <http://purl.org/dc/terms/title> "Wind turbine blade damage ontology"@en ;
                                   <http://purl.org/vocab/vann/preferredNamespacePrefix> "of-bdo" ;
                                   <http://purl.org/vocab/vann/preferredNamespaceUri> "https://w3id.org/ontoforge/bdo#" ;
                                   rdfs:comment "This ontology aims to model Blade damage based on a white paper by EPRI. The ontology is developed in the context of the xxxx project"@en ;
                                   owl:versionInfo "0.0.2" .

#################################################################
#    Annotation properties
#################################################################

###  http://purl.org/dc/terms/creator
<http://purl.org/dc/terms/creator> rdf:type owl:AnnotationProperty .


###  http://purl.org/dc/terms/description
<http://purl.org/dc/terms/description> rdf:type owl:AnnotationProperty .


###  http://purl.org/dc/terms/issued
<http://purl.org/dc/terms/issued> rdf:type owl:AnnotationProperty .


###  http://purl.org/dc/terms/license
<http://purl.org/dc/terms/license> rdf:type owl:AnnotationProperty .


###  http://purl.org/dc/terms/modified
<http://purl.org/dc/terms/modified> rdf:type owl:AnnotationProperty .


###  http://purl.org/dc/terms/publisher
<http://purl.org/dc/terms/publisher> rdf:type owl:AnnotationProperty .


###  http://purl.org/dc/terms/rights
<http://purl.org/dc/terms/rights> rdf:type owl:AnnotationProperty .


###  http://purl.org/dc/terms/title
<http://purl.org/dc/terms/title> rdf:type owl:AnnotationProperty .


###  http://purl.org/vocab/vann/preferredNamespacePrefix
<http://purl.org/vocab/vann/preferredNamespacePrefix> rdf:type owl:AnnotationProperty .


###  http://purl.org/vocab/vann/preferredNamespaceUri
<http://purl.org/vocab/vann/preferredNamespaceUri> rdf:type owl:AnnotationProperty .


###  http://www.w3.org/2004/02/skos/core#definition
<http://www.w3.org/2004/02/skos/core#definition> rdf:type owl:AnnotationProperty .


#################################################################
#    Datatypes
#################################################################

###  http://www.w3.org/2001/XMLSchema#date
xsd:date rdf:type rdfs:Datatype .


#################################################################
#    Object Properties
#################################################################

###  https://w3id.org/ontoforge/bdo#hasDamageCategory
:hasDamageCategory rdf:type owl:ObjectProperty ;
                   rdfs:domain :BladeDamage ;
                   rdfs:range :BladeDamageCategory .


###  https://w3id.org/ontoforge/bdo#hasDamageType
:hasDamageType rdf:type owl:ObjectProperty ;
               rdfs:domain :BladeDamage ;
               rdfs:range :DamageType .


###  https://w3id.org/ontoforge/bdo#requiresAction
:requiresAction rdf:type owl:ObjectProperty ;
                rdfs:domain :BladeDamageCategory ;
                rdfs:range :Procedure .


#################################################################
#    Classes
#################################################################

###  https://w3id.org/ontoforge/bdo#BladeDamage
:BladeDamage rdf:type owl:Class ;
             rdfs:comment "Blade damage."@en ;
             rdfs:label "Blade Damage"@en .


###  https://w3id.org/ontoforge/bdo#BladeDamageCategory
:BladeDamageCategory rdf:type owl:Class ;
                     rdfs:comment "Blade damage category."@en ;
                     rdfs:label "Blade Damage category"@en .


###  https://w3id.org/ontoforge/bdo#DamageType
:DamageType rdf:type owl:Class ;
            rdfs:comment "Blade damage type."@en ;
            rdfs:label "Blade Damage type"@en .


###  https://w3id.org/ontoforge/bdo#Procedure
:Procedure rdf:type owl:Class ;
           rdfs:comment "Proceduree."@en ;
           rdfs:label "Procedure"@en .


#################################################################
#    Individuals
#################################################################

###  https://w3id.org/ontoforge/bdo#AerodynamicPerfomance
:AerodynamicPerfomance rdf:type owl:NamedIndividual ,
                                :DamageType .


###  https://w3id.org/ontoforge/bdo#AerodynamicPerformance_1
:AerodynamicPerformance_1 rdf:type owl:NamedIndividual ,
                                   :BladeDamage ;
                          :hasDamageCategory :BladeDamageCategory2 ;
                          :hasDamageType :AerodynamicPerfomance ;
                          <http://www.w3.org/2004/02/skos/core#definition> "Several missing aerodynamic devices (e.g. vortex generators, trailing edge devices)."@en .


###  https://w3id.org/ontoforge/bdo#AerodynamicPerformance_2
:AerodynamicPerformance_2 rdf:type owl:NamedIndividual ,
                                   :BladeDamage ;
                          :hasDamageCategory :BladeDamageCategory2 ;
                          :hasDamageType :AerodynamicPerfomance ;
                          <http://www.w3.org/2004/02/skos/core#definition> "Heavy dirt, oil, grease, or insects on the blade surface."@en .


###  https://w3id.org/ontoforge/bdo#AerodynamicPerformance_3
:AerodynamicPerformance_3 rdf:type owl:NamedIndividual ,
                                   :BladeDamage ;
                          :hasDamageCategory :BladeDamageCategory2 ;
                          :hasDamageType :AerodynamicPerfomance ;
                          <http://www.w3.org/2004/02/skos/core#definition> "Early stages of leading edge erosion or other increased surface roughness."@en .


###  https://w3id.org/ontoforge/bdo#AerodynamicPerformance_4
:AerodynamicPerformance_4 rdf:type owl:NamedIndividual ,
                                   :BladeDamage ;
                          :hasDamageCategory :BladeDamageCategory3 ;
                          :hasDamageType :AerodynamicPerfomance ;
                          <http://www.w3.org/2004/02/skos/core#definition> "Extensive missing aerodynamic devices (e.g., vortex generators, trailing edge devices)."@en .


###  https://w3id.org/ontoforge/bdo#BladeDamageCategory1
:BladeDamageCategory1 rdf:type owl:NamedIndividual ,
                               :BladeDamageCategory ;
                      :requiresAction :MonitoringBladeDamageCategory1 ,
                                      :OperationBladeDamageCategory1 ,
                                      :RepairBladeDamageCategory1 ;
                      <http://www.w3.org/2004/02/skos/core#definition> "Minor variances from supply specifications but within acceptable (or industry typical) tolerances; may affect the appearance of the blade or blade feature. Though minor, can be useful to identify as position references, or for blade identification."@en .


###  https://w3id.org/ontoforge/bdo#BladeDamageCategory2
:BladeDamageCategory2 rdf:type owl:NamedIndividual ,
                               :BladeDamageCategory ;
                      :requiresAction :MonitoringBladeDamageCategory2 ,
                                      :OperationBladeDamageCategory3 ,
                                      :RepairBladeDamageCategory2 ;
                      <http://www.w3.org/2004/02/skos/core#definition> "Minor damage or defects that exceed supply specification acceptance criteria. Multiple cosmetic findings and/or a single major cosmetic finding that are damage, defects, or former repairs. Findings exceed tolerances of supply conditions or industry typical manufacturing variability. Repairs of more severe damage or defects can be recategorized to category 2 upon review of repair."@en .


###  https://w3id.org/ontoforge/bdo#BladeDamageCategory3
:BladeDamageCategory3 rdf:type owl:NamedIndividual ,
                               :BladeDamageCategory ;
                      :requiresAction :MonitoringBladeDamageCategory3 ,
                                      :OperationBladeDamageCategory3 ,
                                      :RepairBladeDamageCategory3 ;
                      <http://www.w3.org/2004/02/skos/core#definition> """Moderate to minor structural damage or minor manufacturing defects in non-critical areas. Features are moderately out of compliance with supply conditions and/or below minimum typical industry practice. May present as surface indications when in fact there is damage to the underlying structural laminate. Internal inspection may be needed to determine the extent of the finding.
May be particularly challenging to assess criticality due to lack of design data such as load margins. Findings may be category 3 when category 4 actions seem too drastic and category 2 is not appropriate, because there is a slight risk of loss of structural capability."""@en .


###  https://w3id.org/ontoforge/bdo#BladeDamageCategory4
:BladeDamageCategory4 rdf:type owl:NamedIndividual ,
                               :BladeDamageCategory ;
                      :requiresAction :MonitoringBladeDamageCategory4 ,
                                      :OperationBladeDamageCategory4 ,
                                      :RepairBladeDamageCategory4 ;
                      <http://www.w3.org/2004/02/skos/core#definition> "Significant damage or defects that have notable impact to structural capability and/or aerodynamic performance."@en .


###  https://w3id.org/ontoforge/bdo#BladeDamageCategory5
:BladeDamageCategory5 rdf:type owl:NamedIndividual ,
                               :BladeDamageCategory ;
                      :requiresAction :MonitoringBladeDamageCategory5 ,
                                      :OperationBladeDamageCategory5 ,
                                      :RepairBladeDamageCategory5 ;
                      <http://www.w3.org/2004/02/skos/core#definition> "Severe degree of damage or defect such that there is a high risk of imminent failure."@en .


###  https://w3id.org/ontoforge/bdo#CosmeticDamage
:CosmeticDamage rdf:type owl:NamedIndividual ,
                         :DamageType .


###  https://w3id.org/ontoforge/bdo#CosmeticDamage_1
:CosmeticDamage_1 rdf:type owl:NamedIndividual ,
                           :BladeDamage ;
                  :hasDamageCategory :BladeDamageCategory1 ;
                  :hasDamageType :CosmeticDamage ;
                  <http://www.w3.org/2004/02/skos/core#definition> "Marks from small mold positioning devices."@en .


###  https://w3id.org/ontoforge/bdo#CosmeticDamage_2
:CosmeticDamage_2 rdf:type owl:NamedIndividual ,
                           :BladeDamage ;
                  :hasDamageCategory :BladeDamageCategory1 ;
                  :hasDamageType :CosmeticDamage ;
                  <http://www.w3.org/2004/02/skos/core#definition> "Small or thin foreign objects in laminate that do not form wrinkles."@en .


###  https://w3id.org/ontoforge/bdo#CosmeticDamage_3
:CosmeticDamage_3 rdf:type owl:NamedIndividual ,
                           :BladeDamage ;
                  :hasDamageCategory :BladeDamageCategory1 ;
                  :hasDamageType :CosmeticDamage ;
                  <http://www.w3.org/2004/02/skos/core#definition> "Minor variability in thickness of coatings, detectable as translucence."@en .


###  https://w3id.org/ontoforge/bdo#CosmeticDamage_4
:CosmeticDamage_4 rdf:type owl:NamedIndividual ,
                           :BladeDamage ;
                  :hasDamageCategory :BladeDamageCategory1 ;
                  :hasDamageType :CosmeticDamage ;
                  <http://www.w3.org/2004/02/skos/core#definition> "Minor blade surface variability due to mold features."@en .


###  https://w3id.org/ontoforge/bdo#CosmeticDamage_5
:CosmeticDamage_5 rdf:type owl:NamedIndividual ,
                           :BladeDamage ;
                  :hasDamageCategory :BladeDamageCategory1 ;
                  :hasDamageType :CosmeticDamage ;
                  <http://www.w3.org/2004/02/skos/core#definition> "Light dirt, oil, grease, or insects on the blade surface."@en .


###  https://w3id.org/ontoforge/bdo#CosmeticDamage_6
:CosmeticDamage_6 rdf:type owl:NamedIndividual ,
                           :BladeDamage ;
                  :hasDamageCategory :BladeDamageCategory1 ;
                  :hasDamageType :CosmeticDamage ;
                  <http://www.w3.org/2004/02/skos/core#definition> "Missing or unreadable labels or stickers."@en .


###  https://w3id.org/ontoforge/bdo#CosmeticDamage_7
:CosmeticDamage_7 rdf:type owl:NamedIndividual ,
                           :BladeDamage ;
                  :hasDamageCategory :BladeDamageCategory2 ;
                  :hasDamageType :CosmeticDamage ;
                  <http://www.w3.org/2004/02/skos/core#definition> "Coating discoloration, scratches, or cracks, profile deviations in repairs, mold marks protruding from the blade surface, rough paint patches."@en .


###  https://w3id.org/ontoforge/bdo#CosmeticDamage_8
:CosmeticDamage_8 rdf:type owl:NamedIndividual ,
                           :BladeDamage ;
                  :hasDamageCategory :BladeDamageCategory2 ;
                  :hasDamageType :CosmeticDamage ;
                  <http://www.w3.org/2004/02/skos/core#definition> "Thin or flaking coating."@en .


###  https://w3id.org/ontoforge/bdo#CosmeticDamage_9
:CosmeticDamage_9 rdf:type owl:NamedIndividual ,
                           :BladeDamage ;
                  :hasDamageCategory :BladeDamageCategory2 ;
                  :hasDamageType :CosmeticDamage ;
                  <http://www.w3.org/2004/02/skos/core#definition> "Excessive oil on the internal surfaces of the blade."@en .


###  https://w3id.org/ontoforge/bdo#Defect
:Defect rdf:type owl:NamedIndividual ,
                 :DamageType .


###  https://w3id.org/ontoforge/bdo#Defect_1
:Defect_1 rdf:type owl:NamedIndividual ,
                   :BladeDamage ;
          :hasDamageCategory :BladeDamageCategory2 ;
          :hasDamageType :Defect ;
          <http://www.w3.org/2004/02/skos/core#definition> "Minor foreign objects in laminate resulting in small wrinkles."@en .


###  https://w3id.org/ontoforge/bdo#Defect_2
:Defect_2 rdf:type owl:NamedIndividual ,
                   :BladeDamage ;
          :hasDamageCategory :BladeDamageCategory2 ;
          :hasDamageType :Defect ;
          <http://www.w3.org/2004/02/skos/core#definition> "Minor manufacturing deviations that have been evaluated by an engineer and do not impact structural capability due to design margins or it is in an area of low structural criticality."@en .


###  https://w3id.org/ontoforge/bdo#Defect_3
:Defect_3 rdf:type owl:NamedIndividual ,
                   :BladeDamage ;
          :hasDamageCategory :BladeDamageCategory4 ;
          :hasDamageType :Defect ;
          <http://www.w3.org/2004/02/skos/core#definition> "Chordwise wrinkles of laminate fibers in highly loaded regions."@en .


###  https://w3id.org/ontoforge/bdo#Defect_4
:Defect_4 rdf:type owl:NamedIndividual ,
                   :BladeDamage ;
          :hasDamageCategory :BladeDamageCategory4 ;
          :hasDamageType :Defect ;
          <http://www.w3.org/2004/02/skos/core#definition> "Significant areas of underinfused or improperly cured laminate."@en .


###  https://w3id.org/ontoforge/bdo#Defect_5
:Defect_5 rdf:type owl:NamedIndividual ,
                   :BladeDamage ;
          :hasDamageCategory :BladeDamageCategory4 ;
          :hasDamageType :Defect ;
          <http://www.w3.org/2004/02/skos/core#definition> "Large gaps or underbite/overbite at shell bonded joints."@en .


###  https://w3id.org/ontoforge/bdo#Defect_6
:Defect_6 rdf:type owl:NamedIndividual ,
                   :BladeDamage ;
          :hasDamageCategory :BladeDamageCategory4 ;
          :hasDamageType :Defect ;
          <http://www.w3.org/2004/02/skos/core#definition> "Significant missing adhesive bond material, cavities, voids, or cracks in adhesive bonds, or significant deviations of the geometry of adhesive bonds beyond allowable limits."@en .


###  https://w3id.org/ontoforge/bdo#Defect_7
:Defect_7 rdf:type owl:NamedIndividual ,
                   :BladeDamage ;
          :hasDamageCategory :BladeDamageCategory4 ;
          :hasDamageType :Defect ;
          <http://www.w3.org/2004/02/skos/core#definition> "Large foreign objects in laminates that result in significant wrinkles."@en .


###  https://w3id.org/ontoforge/bdo#LightningDamage
:LightningDamage rdf:type owl:NamedIndividual ,
                          :DamageType .


###  https://w3id.org/ontoforge/bdo#LightningDamage_1
:LightningDamage_1 rdf:type owl:NamedIndividual ,
                            :BladeDamage ;
                   :hasDamageCategory :BladeDamageCategory2 ;
                   :hasDamageType :LightningDamage ;
                   <http://www.w3.org/2004/02/skos/core#definition> "Pin holes or very small marks on the blade shell where lightning was intercepted (not at the lightning receptor)."@en .


###  https://w3id.org/ontoforge/bdo#LightningDamage_2
:LightningDamage_2 rdf:type owl:NamedIndividual ,
                            :BladeDamage ;
                   :hasDamageCategory :BladeDamageCategory4 ;
                   :hasDamageType :LightningDamage ;
                   <http://www.w3.org/2004/02/skos/core#definition> "Laminate damage where lightning attached to blade surface, not at the intended receptor."@en .


###  https://w3id.org/ontoforge/bdo#LightningDamage_3
:LightningDamage_3 rdf:type owl:NamedIndividual ,
                            :BladeDamage ;
                   :hasDamageCategory :BladeDamageCategory4 ;
                   :hasDamageType :LightningDamage ;
                   <http://www.w3.org/2004/02/skos/core#definition> "Lightning penetrated the shell, however the exterior surface appears structurally adequate."@en .


###  https://w3id.org/ontoforge/bdo#MechanicalDamage
:MechanicalDamage rdf:type owl:NamedIndividual ,
                           :DamageType .


###  https://w3id.org/ontoforge/bdo#MonitoringBladeDamageCategory1
:MonitoringBladeDamageCategory1 rdf:type owl:NamedIndividual ,
                                         :Procedure ;
                                <http://www.w3.org/2004/02/skos/core#definition> "None needed."@en .


###  https://w3id.org/ontoforge/bdo#MonitoringBladeDamageCategory2
:MonitoringBladeDamageCategory2 rdf:type owl:NamedIndividual ,
                                         :Procedure ;
                                <http://www.w3.org/2004/02/skos/core#definition> "Monitor during routinely scheduled maintenance for damage initiation or progression. Depending on the damage, internal inspection may be warranted to differentiate surface cracks from more severe laminate damage."@en .


###  https://w3id.org/ontoforge/bdo#MonitoringBladeDamageCategory3
:MonitoringBladeDamageCategory3 rdf:type owl:NamedIndividual ,
                                         :Procedure ;
                                <http://www.w3.org/2004/02/skos/core#definition> "Inspection frequency driven by assessment of risk; may be more frequent than routinely scheduled inspections recommended by the OEM. If no growth in damage over time, an engineering assessment may downgrade finding to category 2."@en .


###  https://w3id.org/ontoforge/bdo#MonitoringBladeDamageCategory4
:MonitoringBladeDamageCategory4 rdf:type owl:NamedIndividual ,
                                         :Procedure ;
                                <http://www.w3.org/2004/02/skos/core#definition> "More frequent or more comprehensive monitoring than routine inspections are required until repairs are complete."@en .


###  https://w3id.org/ontoforge/bdo#MonitoringBladeDamageCategory5
:MonitoringBladeDamageCategory5 rdf:type owl:NamedIndividual ,
                                         :Procedure ;
                                <http://www.w3.org/2004/02/skos/core#definition> "If repair is implemented, repair should be deemed a Category 3 defect until sufficient operating experience is gained to provide confidence that the repair is sufficient to achieve expected remaining operating life."@en .


###  https://w3id.org/ontoforge/bdo#OperationBladeDamageCategory1
:OperationBladeDamageCategory1 rdf:type owl:NamedIndividual ,
                                        :Procedure ;
                               <http://www.w3.org/2004/02/skos/core#definition> "Continued operation is possible."@en .


###  https://w3id.org/ontoforge/bdo#OperationBladeDamageCategory2
:OperationBladeDamageCategory2 rdf:type owl:NamedIndividual ,
                                        :Procedure ;
                               <http://www.w3.org/2004/02/skos/core#definition> "Continued operation."@en .


###  https://w3id.org/ontoforge/bdo#OperationBladeDamageCategory3
:OperationBladeDamageCategory3 rdf:type owl:NamedIndividual ,
                                        :Procedure ;
                               <http://www.w3.org/2004/02/skos/core#definition> "Continued operation is possible."@en .


###  https://w3id.org/ontoforge/bdo#OperationBladeDamageCategory4
:OperationBladeDamageCategory4 rdf:type owl:NamedIndividual ,
                                        :Procedure ;
                               <http://www.w3.org/2004/02/skos/core#definition> "Engineering evaluation required to deem blade can operate until repair is scheduled. Operation shall stop if repair cannot be implemented within the allowable time period."@en .


###  https://w3id.org/ontoforge/bdo#OperationBladeDamageCategory5
:OperationBladeDamageCategory5 rdf:type owl:NamedIndividual ,
                                        :Procedure ;
                               <http://www.w3.org/2004/02/skos/core#definition> "The blade is not safe to operate until the damage or defect is repaired or the blade is replaced."@en .


###  https://w3id.org/ontoforge/bdo#RepairBladeDamageCategory1
:RepairBladeDamageCategory1 rdf:type owl:NamedIndividual ,
                                     :Procedure ;
                            <http://www.w3.org/2004/02/skos/core#definition> "None needed, though some can be remedied with minimal effort in conjunction with other blade maintenance activities."@en .


###  https://w3id.org/ontoforge/bdo#RepairBladeDamageCategory2
:RepairBladeDamageCategory2 rdf:type owl:NamedIndividual ,
                                     :Procedure ;
                            <http://www.w3.org/2004/02/skos/core#definition> "Repair is perfomed based on cost/benefit analysis."@en .


###  https://w3id.org/ontoforge/bdo#RepairBladeDamageCategory3
:RepairBladeDamageCategory3 rdf:type owl:NamedIndividual ,
                                     :Procedure ;
                            <http://www.w3.org/2004/02/skos/core#definition> "Repair is performed based on circumstances, criticality, and O&M approach. If found during manufacturing, should be repaired prior to installation. Investigation and repair or replacement of missing aerodynamic devices should be performed to regain energy capture benefits. Timing of repairs can be linked to other blade-related needs. Leading edge erosion or small external cracks should be repaired to prevent damage progression."@en .


###  https://w3id.org/ontoforge/bdo#RepairBladeDamageCategory4
:RepairBladeDamageCategory4 rdf:type owl:NamedIndividual ,
                                     :Procedure ;
                            <http://www.w3.org/2004/02/skos/core#definition> "Repair within a limited number of months of initial observation. Repairs may be performed uptower or blade should be repaired prior to installation and a manufacturing quality assessment should be undertaken to find and correct root causes."@en .


###  https://w3id.org/ontoforge/bdo#RepairBladeDamageCategory5
:RepairBladeDamageCategory5 rdf:type owl:NamedIndividual ,
                                     :Procedure ;
                            <http://www.w3.org/2004/02/skos/core#definition> "Replace, or repair depending on repair feasibility and cost/benefit relative to replacement."@en .


###  https://w3id.org/ontoforge/bdo#StructuralDamage
:StructuralDamage rdf:type owl:NamedIndividual ,
                           :DamageType .


###  https://w3id.org/ontoforge/bdo#StructuralDamage_1
:StructuralDamage_1 rdf:type owl:NamedIndividual ,
                             :BladeDamage ;
                    :hasDamageCategory :BladeDamageCategory3 ;
                    :hasDamageType :StructuralDamage ;
                    <http://www.w3.org/2004/02/skos/core#definition> "Small cracks in shells or along leading or trailing edge bonds, small areas of underinfused laminate, voids in adhesive bonds."@en .


###  https://w3id.org/ontoforge/bdo#StructuralDamage_10
:StructuralDamage_10 rdf:type owl:NamedIndividual ,
                              :BladeDamage ;
                     :hasDamageCategory :BladeDamageCategory5 ;
                     :hasDamageType :StructuralDamage ;
                     <http://www.w3.org/2004/02/skos/core#definition> "Separation of shear webs from spar caps."@en .


###  https://w3id.org/ontoforge/bdo#StructuralDamage_11
:StructuralDamage_11 rdf:type owl:NamedIndividual ,
                              :BladeDamage ;
                     :hasDamageCategory :BladeDamageCategory5 ;
                     :hasDamageType :StructuralDamage ;
                     <http://www.w3.org/2004/02/skos/core#definition> "Numerous broken blade bolts."@en .


###  https://w3id.org/ontoforge/bdo#StructuralDamage_12
:StructuralDamage_12 rdf:type owl:NamedIndividual ,
                              :BladeDamage ;
                     :hasDamageCategory :BladeDamageCategory5 ;
                     :hasDamageType :StructuralDamage ;
                     <http://www.w3.org/2004/02/skos/core#definition> "Significant chordwise or spanwise cracks or large delaminations in shells."@en .


###  https://w3id.org/ontoforge/bdo#StructuralDamage_2
:StructuralDamage_2 rdf:type owl:NamedIndividual ,
                             :BladeDamage ;
                    :hasDamageCategory :BladeDamageCategory3 ;
                    :hasDamageType :StructuralDamage ;
                    <http://www.w3.org/2004/02/skos/core#definition> "Significant root face laminate wrinkles."@en .


###  https://w3id.org/ontoforge/bdo#StructuralDamage_3
:StructuralDamage_3 rdf:type owl:NamedIndividual ,
                             :BladeDamage ;
                    :hasDamageCategory :BladeDamageCategory3 ;
                    :hasDamageType :StructuralDamage ;
                    <http://www.w3.org/2004/02/skos/core#definition> "Spanwise wrinkles in laminate."@en .


###  https://w3id.org/ontoforge/bdo#StructuralDamage_4
:StructuralDamage_4 rdf:type owl:NamedIndividual ,
                             :BladeDamage ;
                    :hasDamageCategory :BladeDamageCategory4 ;
                    :hasDamageType :StructuralDamage ;
                    <http://www.w3.org/2004/02/skos/core#definition> "Significant cracks, delamination, buckling of shells."@en .


###  https://w3id.org/ontoforge/bdo#StructuralDamage_5
:StructuralDamage_5 rdf:type owl:NamedIndividual ,
                             :BladeDamage ;
                    :hasDamageCategory :BladeDamageCategory4 ;
                    :hasDamageType :StructuralDamage ;
                    <http://www.w3.org/2004/02/skos/core#definition> "Significant lead edge or trailing edge separation, exposing internal structure to water ingress."@en .


###  https://w3id.org/ontoforge/bdo#StructuralDamage_6
:StructuralDamage_6 rdf:type owl:NamedIndividual ,
                             :BladeDamage ;
                    :hasDamageCategory :BladeDamageCategory4 ;
                    :hasDamageType :StructuralDamage ;
                    <http://www.w3.org/2004/02/skos/core#definition> "Moderate to large core gaps or missing core material."@en .


###  https://w3id.org/ontoforge/bdo#StructuralDamage_7
:StructuralDamage_7 rdf:type owl:NamedIndividual ,
                             :BladeDamage ;
                    :hasDamageCategory :BladeDamageCategory4 ;
                    :hasDamageType :StructuralDamage ;
                    <http://www.w3.org/2004/02/skos/core#definition> "Leading edge erosion through shells, exposing blade internal structure."@en .


###  https://w3id.org/ontoforge/bdo#StructuralDamage_8
:StructuralDamage_8 rdf:type owl:NamedIndividual ,
                             :BladeDamage ;
                    :hasDamageCategory :BladeDamageCategory4 ;
                    :hasDamageType :StructuralDamage ;
                    <http://www.w3.org/2004/02/skos/core#definition> "Broken blade bolt."@en .


###  https://w3id.org/ontoforge/bdo#StructuralDamage_9
:StructuralDamage_9 rdf:type owl:NamedIndividual ,
                             :BladeDamage ;
                    :hasDamageCategory :BladeDamageCategory5 ;
                    :hasDamageType :StructuralDamage ;
                    <http://www.w3.org/2004/02/skos/core#definition> "Buckled shear webs."@en .


###  Generated by the OWL API (version 5.1.18) https://github.com/owlcs/owlapi/
